Refactor the correctness of alpha-beta pruning

MinMax.v
@@ -1,4 +1,4 @@
-Require Import List Relations ZArith Omega Program.
+Require Import List Relations ZArith Lia Program ssreflect.
 
 Section Maximum.
   Variable A : Set.
@@ -7,35 +7,21 @@ Section Maximum.
 
   Hypothesis max_select : forall x y, max x y = x \/ max x y = y.
 
-  Theorem maximum_select xs : forall x, In (maximum x xs) (x :: xs).
+  Theorem maximum_select : forall xs x, In (maximum x xs) (x :: xs).
   Proof.
-    induction xs as [ | x xs ]; simpl; intros x'.
-    - eauto.
-    - destruct (max_select x' x) as [ Heq | Heq ];
-        rewrite Heq;
-        [ destruct (IHxs x')
-        | destruct (IHxs x) ];
-        eauto.
+    elim => /= [ | x ? IH x' ]; eauto.
+    case (max_select x' x) => ->; [ case (IH x') | case (IH x) ]; eauto.
   Qed.
 
   Variable le : relation A.
   Hypothesis le_refl : forall x, le x x.
   Hypothesis le_trans : forall x y z, le x y -> le y z -> le x z.
-  Hypothesis max_join : forall x y, le x (max x y) /\ le y (max x y).
+  Hypothesis max_left : forall x y, le x (max x y).
+  Hypothesis max_right : forall x y, le y (max x y).
 
-  Theorem maximum_join xs : forall x y, In y (x :: xs) -> le y (maximum x xs).
+  Theorem maximum_join : forall xs x y, In y (x :: xs) -> le y (maximum x xs).
   Proof.
-    induction xs as [ | x xs ]; simpl.
-    - intros ? ? [ ? | [] ]; subst; eauto.
-    - intros x' y [ ? | [ ? | ? ] ]; subst.
-      + destruct (max_join y x).
-        specialize (IHxs (max y x) _ (or_introl eq_refl)).
-        eauto.
-      + destruct (max_join x' y).
-        specialize (IHxs (max x' y) _ (or_introl eq_refl)).
-        eauto.
-      + apply IHxs; simpl.
-        eauto.
+    elim => /= [ ? ? [ -> | [ ] ] | x xs IHxs x' y [ -> | [ -> | ] ] ]; eauto.
   Qed.
 
   Definition maximum_spec x xs := conj (maximum_select xs x) (maximum_join xs x).
@@ -53,64 +39,36 @@ Section ZMaximum.
   Corollary Zmaximum_spec : forall x xs,
     (In (Zmaximum x xs) (x :: xs)) /\
     (forall y, In y (x :: xs) -> y <= Zmaximum x xs).
-  Proof.
-    apply maximum_spec; try (intros; omega).
-    - intros x y.
-      destruct (Zmax_spec x y) as [[]|[]]; omega. 
-    - intros x y.
-      destruct (Zmax_spec x y) as [[]|[]]; omega.
-  Qed.
+  Proof. by apply /maximum_spec; lia. Qed.
 
   Corollary Zminimum_spec : forall x xs,
     In (Zminimum x xs) (x :: xs) /\
     (forall y, In y (x :: xs) -> y >= Zminimum x xs).
-  Proof.
-    apply maximum_spec; try (intros; omega).
-    - intros x y.
-      destruct (Zmin_spec x y) as [[]|[]]; omega. 
-    - intros x y.
-      destruct (Zmin_spec x y) as [[]|[]]; omega.
-  Qed.
+  Proof. by apply /maximum_spec; lia. Qed.
 
   Corollary neg_Zmaximum_distr x xs :
     - Zmaximum x xs = Zminimum (- x) (map Z.opp xs).
   Proof.
-    destruct (Zmaximum_spec x xs) as [ HmaxIn Hmax ].
-    destruct (Zminimum_spec (- x) (map Z.opp xs)) as [ HminIn Hmin ].
-
-    assert (HmaxIn' : In (- Zmaximum x xs) (map Z.opp (x :: xs))).
-    { apply in_map. eauto. }
-    specialize (Hmin _ HmaxIn').
-
-    assert (HminIn' : In (- Zminimum (- x) (map Z.opp xs)) (map Z.opp (map Z.opp (x :: xs)))).
-    { apply in_map. eauto. }
-    rewrite map_map in HminIn'.
-    rewrite map_ext with (f := fun x => - - x) (g := id) in HminIn'
-      by (unfold id; intros; omega).
-    rewrite map_id in HminIn'.
-    specialize (Hmax _ HminIn').
-
-    omega.
+    case (Zmaximum_spec x xs) => HmaxIn Hmax.
+    case (Zminimum_spec (- x) (map Z.opp xs)) => HminIn Hmin.
+    have /Hmin : In (- Zmaximum x xs) (map Z.opp (x :: xs)) by apply /in_map.
+    have : In (- Zminimum (- x) (map Z.opp xs)) (map Z.opp (map Z.opp (x :: xs))) by apply /in_map.
+    rewrite map_map (map_ext (fun x => - - x) id) /id ?map_id => [ | /Hmax ]; lia.
   Qed.
 
   Corollary neg_Zminimum_distr x xs :
     - Zminimum x xs = Zmaximum (- x) (map Z.opp xs).
   Proof.
-    replace (Zminimum x xs) with (Zminimum (- - x) (map Z.opp (map Z.opp xs))).
-    - rewrite <- neg_Zmaximum_distr.
-      omega.
-    - f_equal.
-      + omega.
-      + rewrite <- map_id.
-        repeat rewrite map_map.
-        apply map_ext.
-        intros.
-        omega.
+    have -> : Zminimum x xs = Zminimum (- - x) (map Z.opp (map Z.opp xs)).
+    { congr (Zminimum _ _).
+      - by lia.
+      - rewrite map_map -(map_ext id) ?map_id // /id. by lia. }
+    rewrite -neg_Zmaximum_distr. by lia.
   Qed.
 
   Corollary Zmaximum_concrete : forall x xs,
     fold_left Z.max xs x = Zmaximum x xs.
-  Proof. apply maximum_concrete. Qed.
+  Proof. exact /maximum_concrete. Qed.
 End ZMaximum.
 
 Section MinMax.
@@ -125,9 +83,9 @@ Section MinMax.
     | O => eval b
     | S n =>
         match succ b with
-        | [] => eval b
+        | nil => eval b
         | b :: bs =>
-            Zmaximum 
+            Zmaximum
               (minimax' b n)
               (map (fun b => minimax' b n) bs)
         end
@@ -137,7 +95,7 @@ Section MinMax.
     | O => eval b
     | S n =>
         match succ b with
-        | [] => eval b
+        | nil => eval b
         | b :: bs =>
             Zminimum
               (minimax b n)
@@ -152,7 +110,7 @@ Section MinMax.
         else - eval b
     | S n =>
         match succ b with
-        | [] =>
+        | nil =>
             if turn then eval b
             else - eval b
         | b :: bs =>
@@ -162,21 +120,14 @@ Section MinMax.
         end
     end.
 
-  Theorem negmax_corresponds_minimax n : forall b turn,
+  Theorem negmax_corresponds_minimax : forall n b turn,
     negmax turn b n = if turn then minimax b n else - minimax' b n.
   Proof.
-    induction n as [ | n ]; simpl.
-    - intros ? []; reflexivity.
-    - intros b0 [];
-        destruct (succ b0); eauto.
-      + rewrite map_map.
-        f_equal; [ | apply map_ext; intros ? ];
-          rewrite (IHn _); simpl;
-          omega.
-      + rewrite <- neg_Zminimum_distr.
-        do 2 f_equal; [ | apply map_ext; intros ? ];
-          rewrite (IHn _); simpl;
-          omega.
+    elim => /= [ ? [ ] | ? IH b [ ] ] //; case (succ b) => // ? ?.
+    - rewrite map_map.
+      congr (Zmaximum _ _); [ | apply /map_ext => ? ]; rewrite IH /=; by lia.
+    - rewrite -neg_Zminimum_distr.
+      congr (- Zminimum _ _); [ | apply /map_ext => ? ]; rewrite IH /=; by lia.
   Qed.
 
   Definition Zmaximum_with_alpha {A} alphabeta alpha beta := (fix Zmaximum_with_alpha alpha (xs : list A) :=
@@ -184,73 +135,65 @@ Section MinMax.
     | nil => alpha
     | x :: xs =>
         let value := alphabeta alpha x in
-        if Z_le_dec beta value then value
-        else Zmaximum_with_alpha (Z.max alpha value) xs
+        match Z_le_dec beta value with
+        | left _ => value
+        | right _ => Zmaximum_with_alpha (Z.max alpha value) xs
+        end
     end) alpha.
 
-  Lemma Zmaximum_with_alpha_spec_aux A minimax alphabeta beta xs :
-    (forall alpha (x : A),
+  Lemma Zmaximum_with_alpha_spec_aux A minimax alphabeta beta
+    (Halphabeta_spec : forall alpha (x : A),
       alpha < beta ->
       minimax x <= alpha /\ alphabeta alpha x <= alpha \/
       alpha <= minimax x /\ minimax x = alphabeta alpha x /\ minimax x < beta \/
-      beta <= minimax x /\ beta <= alphabeta alpha x) ->
-    forall alpha,
+      beta <= minimax x /\ beta <= alphabeta alpha x) :
+    forall xs alpha,
     alpha < beta ->
     fold_left Z.max (map minimax xs) alpha = Zmaximum_with_alpha alphabeta alpha beta xs /\
     fold_left Z.max (map minimax xs) alpha < beta \/
     beta <= fold_left Z.max (map minimax xs) alpha /\ beta <= Zmaximum_with_alpha alphabeta alpha beta xs.
   Proof.
-    intros Halphabeta_spec.
-    induction xs as [ | x xs ]; simpl; intros alpha ?.
-    - omega.
-    - destruct (Halphabeta_spec alpha x) as [ [ ] | [ [ ? [ Heq ] ] | [ ] ]]; eauto.
-      + destruct (Z_le_dec beta (alphabeta alpha x)); [ omega | ].
-        repeat rewrite Z.max_l by assumption.
-        apply IHxs; assumption.
-      + rewrite <- Heq.
-        destruct (Z_le_dec beta (minimax x)); [ omega | ].
-        rewrite Z.max_r by omega.
-        apply IHxs; assumption.
-      + right.
-        destruct (Z_le_dec beta (alphabeta alpha x)); [ | omega ].
-        rewrite Z.max_r by omega.
-        split.
-        * rewrite Zmaximum_concrete.
-          specialize (proj2 (Zmaximum_spec (minimax x) (map minimax xs)) _ (or_introl eq_refl)).
-          omega.
-        * assumption.
+    elim => /= [ | x xs IH alpha ? ].
+    - lia.
+    - case (Halphabeta_spec alpha x) => //= [ [ ? ? ] | [ [ ? [ <- ? ] ] | [ ? ? ] ] ].
+      + case (Z_le_dec beta (alphabeta alpha x)) => ?; try lia.
+        rewrite !Z.max_l; try lia.
+        exact /IH.
+      + case (Z_le_dec beta (minimax x)) => ?; try lia.
+        rewrite !Z.max_r; try lia.
+        exact /IH.
+      + case (Z_le_dec beta (alphabeta alpha x)) => ?; try lia.
+        rewrite Zmaximum_concrete !Z.max_r; try lia.
+        move: (proj2 (Zmaximum_spec (minimax x) (map minimax xs)) _ (or_introl eq_refl)).
+        lia.
   Qed.
 
-  Corollary Zmaximum_with_alpha_spec A minimax alphabeta alpha beta xs :
-    alpha < beta ->
-    (forall alpha (x : A),
+  Corollary Zmaximum_with_alpha_spec A minimax alphabeta alpha beta xs
+    (Halphabeta : alpha < beta)
+    (Halphabeta_spec : forall alpha (x : A),
       alpha < beta ->
       minimax x <= alpha /\ alphabeta alpha x <= alpha \/
       alpha <= minimax x /\ minimax x = alphabeta alpha x /\ minimax x < beta \/
-      beta <= minimax x /\ beta <= alphabeta alpha x) ->
+      beta <= minimax x /\ beta <= alphabeta alpha x) :
     alpha <= Zmaximum alpha (map minimax xs) /\
     Zmaximum alpha (map minimax xs) = Zmaximum_with_alpha alphabeta alpha beta xs /\
     Zmaximum alpha (map minimax xs) < beta \/
     beta <= Zmaximum alpha (map minimax xs) /\ beta <= Zmaximum_with_alpha alphabeta alpha beta xs.
   Proof.
-    intros Halphabeta Halphabeta_spec.
-    rewrite <- Zmaximum_concrete.
-    destruct (Zmaximum_with_alpha_spec_aux _ _ _ _ xs Halphabeta_spec _ Halphabeta) as [ [ ] | [ ] ];
-      [ left | right ];
-      repeat split; eauto.
+    rewrite -Zmaximum_concrete.
+    move: (Zmaximum_with_alpha_spec_aux _ _ _ _ Halphabeta_spec xs _ Halphabeta) => [ ] [ ? ? ]; [ left | right ]; repeat split; eauto.
     rewrite Zmaximum_concrete.
-    apply (proj2 (Zmaximum_spec _ _)). left.
-    eauto.
+    apply /(proj2 (Zmaximum_spec _ _)). by left.
   Qed.
 
   Fixpoint alphabeta (turn : bool) alpha beta b n :=
     match n with
-    | O => 
+    | O =>
         if turn then eval b
         else - eval b
     | S n =>
         match succ b with
-        | [] => 
+        | nil =>
             if turn then eval b
             else - eval b
         | bs =>
@@ -268,40 +211,24 @@ Section MinMax.
     negmax turn b n < beta \/
     beta <= negmax turn b n /\ beta <= alphabeta turn alpha beta b n.
   Proof.
-    intros n.
-    induction n as [ | n ]; simpl; intros b beta.
-    - intros; omega.
-    - destruct (succ b) as [ | b_ bs ]; intros turn alpha ?.
-      + omega.
-      + rewrite map_map.
-        destruct (Z_lt_dec alpha (Zmaximum (- negmax (negb turn) b_ n)
-          (map (fun b => - negmax (negb turn) b n) bs))) as [ | ].
-        * right.
-          replace (Zmaximum (- negmax (negb turn) b_ n) (map (fun x => - negmax (negb turn) x n) bs))
-             with (Zmaximum alpha (map (fun x => - negmax (negb turn) x n) (b_ :: bs))).
-          { apply (Zmaximum_with_alpha_spec _ _
-              (fun alpha b => - alphabeta (negb turn) (- beta) (- alpha) b n) _ beta (b_ :: bs)); eauto.
-            intros alpha0 b0 ?.
-            destruct (IHn b0 (- alpha0) (negb turn) (- beta)) as [ [] | [ [ ? [] ] | [ ] ] ]; omega. }
-          { destruct (Zmaximum_spec (- negmax (negb turn) b_ n) (map (fun b => - negmax (negb turn) b n) bs)) as [ HIn1 Hmax1 ].
-            destruct (Zmaximum_spec alpha (map (fun b => - negmax (negb turn) b n) (b_ :: bs))) as [ [ | HIn2 ] Hmax2 ];
-              specialize (Hmax2 _ (or_intror HIn1)).
-            - omega.
-            - specialize (Hmax1 _ HIn2).
-              omega. }
-        * left.
-          assert (Zmaximum alpha (map (fun b => - negmax (negb turn) b n) (b_ :: bs)) = alpha).
-          { destruct (Zmaximum_spec (- negmax (negb turn) b_ n) (map (fun b => - negmax (negb turn) b n) bs)) as [ HIn1 Hmax1 ].
-            destruct (Zmaximum_spec alpha (map (fun b => - negmax (negb turn) b n) (b_ :: bs))) as [ [ | HIn2 ] Hmax2 ].
-            - omega.
-            - generalize (Hmax2 _ (or_intror HIn1)). intros.
-              specialize (Hmax2 _ (or_introl eq_refl)).
-              specialize (Hmax1 _ HIn2).
-              omega. }
-          destruct (Zmaximum_with_alpha_spec _
-            (fun b => - negmax (negb turn) b n)
-            (fun alpha b => - alphabeta (negb turn) (- beta) (- alpha) b n) alpha beta (b_ :: bs)) as [ [ ? [ ] ] | [ ] ]; simpl in *; try omega.
-          intros alpha0 b0 ?.
-          destruct (IHn b0 (- alpha0) (negb turn) (- beta)) as [ [] | [ [ ? [] ] | [ ] ] ]; omega.
+    elim => /= [ | n IHn b beta ]; try lia.
+    case (succ b) => [ | b_ bs ] turn alpha ?; try lia.
+    rewrite map_map.
+    case (Z_lt_dec alpha (Zmaximum (- negmax (negb turn) b_ n) (map (fun b => - negmax (negb turn) b n) bs))) => ?.
+    - right.
+      have -> : Zmaximum (- negmax (negb turn) b_ n) (map (fun x => - negmax (negb turn) x n) bs) = Zmaximum alpha (map (fun x => - negmax (negb turn) x n) (b_ :: bs)).
+      { case (Zmaximum_spec (- negmax (negb turn) b_ n) (map (fun b => - negmax (negb turn) b n) bs)) => HIn1 Hmax1.
+        case (Zmaximum_spec alpha (map (fun b => - negmax (negb turn) b n) (b_ :: bs))) => [ [ ? | HIn2 ] Hmax2 ]; have := Hmax2 _ (or_intror HIn1); [ | have := (Hmax1 _ HIn2) ]; lia. }
+      { apply /(Zmaximum_with_alpha_spec _ _ (fun alpha b => - alphabeta (negb turn) (- beta) (- alpha) b n) _ beta (b_ :: bs)) => // alpha0 b0 ?.
+        case (IHn b0 (- alpha0) (negb turn) (- beta)) => [ | [ ] | [ [ ? [ ] ] | [ ] ] ]; lia. }
+    - left.
+      have : Zmaximum alpha (map (fun b => - negmax (negb turn) b n) (b_ :: bs)) = alpha.
+      { case (Zmaximum_spec (- negmax (negb turn) b_ n) (map (fun b => - negmax (negb turn) b n) bs)) => HIn1 Hmax1.
+        case (Zmaximum_spec alpha (map (fun b => - negmax (negb turn) b n) (b_ :: bs))) => [ [ | HIn2 ] Hmax2 ];
+        [ | move: (Hmax2 _ (or_intror HIn1)) (Hmax2 _ (or_introl eq_refl)) (Hmax1 _ HIn2) ]; lia. }
+      case (Zmaximum_with_alpha_spec _
+        (fun b => - negmax (negb turn) b n)
+        (fun alpha b => - alphabeta (negb turn) (- beta) (- alpha) b n) alpha beta (b_ :: bs)) => /= [ | alpha0 b0 ? | | ]; try lia.
+      case (IHn b0 (- alpha0) (negb turn) (- beta)) => [ | [ ] | [ [ ? [ ] ] | [ ] ] ]; lia.
   Qed.
 End MinMax.
